{
 "cells": [
  {
   "cell_type": "markdown",
   "metadata": {},
   "source": [
    "# Model\n",
    "$$\n",
    "\\begin{align}\n",
    "p(\\boldsymbol{Y},\\boldsymbol{Z},\\boldsymbol{S},\\boldsymbol{\\Lambda},\\boldsymbol{R},\\boldsymbol{\\pi})=&p(\\boldsymbol{Y}|\\boldsymbol{Z},\\boldsymbol{S},\\boldsymbol{\\Lambda},\\boldsymbol{R})p(\\boldsymbol{Z})p(\\boldsymbol{S}|\\boldsymbol{\\pi})p(\\boldsymbol{\\Lambda})p(\\boldsymbol{R})p(\\boldsymbol{\\pi})\n",
    "\\\\\n",
    "p(\\boldsymbol{Y}|\\boldsymbol{Z},\\boldsymbol{S},\\boldsymbol{\\Lambda},\\boldsymbol{R})&=\\prod_{t=1}^T\\prod_{d=1}^D\\prod_{k=1}^K\\mathcal{N}(\\boldsymbol{y}_{d,t}|\\boldsymbol{\\Lambda}_d^{(k)^T}\\boldsymbol{z}_t,\\boldsymbol{R}_d^{(k)^{−1}})^{s_t^{(k)}}\n",
    "\\\\\n",
    "p(\\boldsymbol{S}|\\boldsymbol{\\pi})&=\\prod_{t=1}^{T}\\mathrm{Cat}(s_t|\\boldsymbol{\\pi})\n",
    "\\\\\n",
    "p(\\boldsymbol{\\Lambda})&=\\prod_{d=1}^{D}\\prod_{k=1}^{K}\\mathcal{N}(\\boldsymbol{\\Lambda}_d^{(k)}|\\boldsymbol{\\mu}^{(k)}_{\\boldsymbol{\\Lambda}_d},\\boldsymbol{\\Sigma}^{(k)}_{\\boldsymbol{\\Lambda}_d})\n",
    "\\\\\n",
    "p(\\boldsymbol{R})&=\\prod_{d=1}^{D}\\prod_{k=1}^{K}\\mathrm{Gam}(\\boldsymbol{R}_{d}^{(k)}|a_{R_d}^{(k)},b_{R_d}^{(k)})\n",
    "\\\\\n",
    "p(\\boldsymbol{Z})&=\\prod_t^T \\mathcal{N}(z_{t}|\\mu_{z},\\Sigma_{z})=\\prod_t^T \\prod_{l=1}^{L + 1} \\mathcal{N} (z_{l,t}|\\mu_{z_l},\\sigma_{z_l}^2)\n",
    "\\\\\n",
    "&\\mu_{z_l}=\\left\\{\\begin{matrix}\n",
    "0,&l&=& 1,\\cdots,L\n",
    "\\\\\n",
    "1,&l&=&L + 1\n",
    "\\end{matrix}\\right.\n",
    "\\\\\n",
    "&\\sigma_{z_l}^{2}=\\left\\{\\begin{matrix}\n",
    "1,&l&=&1,\\cdots,L\n",
    "\\\\\n",
    "\\epsilon,&l&=&L+1 \n",
    "\\end{matrix}\\right.\n",
    "\\end{align}\n",
    "$$\n",
    "(R is diagonal)\n",
    "\n"
   ]
  },
  {
   "cell_type": "markdown",
   "metadata": {},
   "source": [
    "# Variational Inference\n",
    "\n",
    "$$\n",
    "\\begin{align}\n",
    "p(\\boldsymbol{Z},\\boldsymbol{S},\\boldsymbol{\\Lambda},\\boldsymbol{R},\\boldsymbol{\\pi}) \\approx & q(\\boldsymbol{Z},\\boldsymbol{S})q(\\boldsymbol{\\Lambda})q(\\boldsymbol{R})q(\\boldsymbol{\\pi})\n",
    "\\\\\n",
    "\\ln p(\\boldsymbol{Z},\\boldsymbol{S}) &= \\langle \\ln p(\\boldsymbol{Y}|\\boldsymbol{Z},\\boldsymbol{S},\\boldsymbol{\\Lambda},\\boldsymbol{R})\\rangle_{q(\\boldsymbol{\\Lambda},\\boldsymbol{R})}+ \\ln p(\\boldsymbol{Z})+\\langle p(\\boldsymbol{S}|\\boldsymbol{\\pi})\\rangle_{q(\\boldsymbol{\\pi})} + C\n",
    "\\\\\n",
    "\\ln q(\\boldsymbol{\\Lambda})&=\\langle \\ln p(\\boldsymbol{Y}|\\boldsymbol{Z},\\boldsymbol{S},\\boldsymbol{\\Lambda},\\boldsymbol{R})\\rangle_{q(\\boldsymbol{Z},\\boldsymbol{S}),q(\\boldsymbol{R})}+\\ln p(\\boldsymbol{\\Lambda})+C\n",
    "\\\\\n",
    "\\ln q(\\boldsymbol{R})&=\\langle \\ln p(\\boldsymbol{Y}|\\boldsymbol{Z},\\boldsymbol{S},\\boldsymbol{\\Lambda},\\boldsymbol{R})\\rangle_{q(\\boldsymbol{Z},\\boldsymbol{S}),q(\\boldsymbol{\\Lambda})}+\\ln q(\\boldsymbol{R})+C\n",
    "\\\\\n",
    "\\ln q(\\boldsymbol{\\pi})&=\\langle\\ln p(\\boldsymbol{S}|\\boldsymbol{\\pi})\\rangle_{q(\\boldsymbol{S})}+\\ln p(\\boldsymbol{\\pi}) +C\n",
    "\\end{align}\n",
    "$$\n"
   ]
  },
  {
   "cell_type": "markdown",
   "metadata": {},
   "source": [
    "# q(Z,S)\n",
    "$$\n",
    "\\begin{align}\n",
    "\\ln p(\\boldsymbol{Z},\\boldsymbol{S}) =& \\langle \\ln p(\\boldsymbol{Y}|\\boldsymbol{Z},\\boldsymbol{S},\\boldsymbol{\\Lambda},\\boldsymbol{R})\\rangle_{q(\\boldsymbol{\\Lambda},\\boldsymbol{R})}+ \\ln p(\\boldsymbol{Z})+\\langle p(\\boldsymbol{S}|\\boldsymbol{\\pi})\\rangle_{q(\\boldsymbol{\\pi})} + C\n",
    "\\\\\n",
    "=&\\sum_{t=1}^{T}\\sum_{k=1}^{K}\\sum_{d=1}^{D}−\\frac{1}{2}s_t^{(k)}\\langle \\{(y_{d,t} − \\boldsymbol{\\Lambda}_d^{(k)^T} \\boldsymbol{z}_t^{(k)})^2 R^{(k)}_d-\\ln R^{(k)}_d+D\\ln 2\\pi\\}\\rangle \n",
    "\\\\\n",
    "&+\\sum_{t=1}^{T}\\sum_{k=1}^{K}(\\boldsymbol{z}^{(k)}_{t} - \\boldsymbol{\\mu}_{z})^T \\boldsymbol{\\Sigma}_{z}^{-1} (\\boldsymbol{z}^{(k)}_{t} - \\boldsymbol{\\mu}_{z})+\\ln |\\boldsymbol{\\Sigma}_z| + L \\ln 2\\pi \n",
    "\\\\\n",
    "&+ \\sum_{t=1}^{T}\\sum_{k=1}^{K} s_t^{(k)}\\langle\\ln\\pi^{(k)}\\rangle +C\n",
    "\\\\\n",
    "=&\\sum_{t=1}^{T}\\sum_{k=1}^{K}\\sum_{d=1}^{D}−\\frac{1}{2}s_t^{(k)} \\{(y_{d,t}^2 \\langle R^{(k)}_d \\rangle − 2 y_{d,t}\\langle\\boldsymbol{\\Lambda}_d^{(k)^T}\\rangle \\boldsymbol{z}_t^{(k)}\\langle R^{(k)}_d\\rangle + (\\langle \\boldsymbol{\\Lambda}_d^{(k)^T}\\rangle \\boldsymbol{z}_t^{(k)})(\\langle \\boldsymbol{ \\Lambda}_d^{(k)^T}\\rangle  \\boldsymbol{z}_t^{(k)})\\langle R^{(k)}_d \\rangle-\\langle \\ln R^{(k)}_d\\rangle +D\\ln 2\\pi\\}\n",
    "\\\\\n",
    "&+\\sum_{t=1}^{T}\\sum_{k=1}^{K}\\boldsymbol{z}^{(k)^T}_{t} \\boldsymbol{\\Sigma}_{z}^{-1}\\boldsymbol{z}^{(k)}_{t} - 2 \\boldsymbol{z}^{(k)^T}_{t} \\boldsymbol{\\Sigma}_{z}^{-1}\\boldsymbol{\\mu}_{z} + \\boldsymbol{\\mu}_{z}^T \\boldsymbol{\\Sigma}_{z}^{-1}\\boldsymbol{\\mu}_{z}+\\ln |\\boldsymbol{\\Sigma}_z| + L \\ln 2\\pi \n",
    "\\\\\n",
    "&+ \\sum_{t=1}^{T}\\sum_{k=1}^{K} s_t^{(k)}\\langle\\ln\\pi^{(k)}\\rangle +C\n",
    "\\\\\n",
    "=& \\ln q(\\boldsymbol{Z}|\\boldsymbol{S}) + \\ln q(\\boldsymbol{S})\n",
    "\\end{align}\n",
    "$$\n",
    "## q(Z|S)\n",
    "$$\n",
    "\\begin{align}\n",
    "\\ln q(\\boldsymbol{Z}|\\boldsymbol{S})=& \\sum_{t=1}^{T}\\sum_{k=1}^{K} s_t^{(k)} \\mathcal{N}(\\boldsymbol{z}_t^{(k)}|\\hat{\\boldsymbol{\\mu}}_z^{(k)}, \\hat{\\boldsymbol{\\Sigma}}_z^{(k)}) + C\n",
    "\\\\\n",
    "&\\hat{\\boldsymbol{\\Sigma}}_z^{(k)^{-1}}=\\boldsymbol{\\Sigma}_z^{-1} + \\Sigma_{d=1}^{D} \\langle \\boldsymbol{\\Lambda}_d^{(k)}\\boldsymbol{\\Lambda}_d^{(k)^T}\\rangle\\langle R_d^{(k)}\\rangle\n",
    "\\\\\n",
    "&\\hat{\\boldsymbol{\\mu}}_z^{(k)}=\\hat{\\boldsymbol{\\Sigma}}_z^{(k)}[\\Sigma_{d=1}^{D} y_{d,t}\\langle R_d^{(k)}\\rangle\\langle\\boldsymbol{\\Lambda}_d^{(k)}\\rangle +\\boldsymbol{\\Sigma}_z^{-1}\\boldsymbol{\\mu}_z]\n",
    "\\end{align}\n",
    "$$\n",
    "## q(S)\n",
    "$$\n",
    "\\begin{align}\n",
    "\\ln q(\\boldsymbol{S})=& \\sum_{t=1}^{T}\\mathrm{Cat}(\\boldsymbol{s}_t|\\hat{\\boldsymbol{\\alpha}}_{\\pi}) + C\n",
    "\\\\\n",
    "\\hat{\\eta}&\\propto \\exp[-\\frac{1}{2}\\{\\sum_{d=1}^D y_{d,t}^2 \\langle R_d^{(k)}\\rangle - \\sum_{d=1}^D \\langle \\ln R_d^{(k)}\\rangle + \\boldsymbol{\\mu_{z}}^T\\boldsymbol{\\Sigma}_{z}^{-1}\\boldsymbol{\\mu}_{z}+\\hat{\\boldsymbol{\\mu}}_{z_t}^{(k)^T}\\hat{\\boldsymbol{\\Sigma}}_{z}^{-1}\\hat{\\boldsymbol{\\mu}}_{z_t}^{(k)}+\\ln|\\boldsymbol{\\Sigma}_{z}|+\\ln|\\hat{\\boldsymbol{\\Sigma}}_{z}|+D\\ln 2\\pi+\\}\\langle \\ln \\pi_k\\rangle]\n",
    "\\end{align}\n",
    "$$"
   ]
  },
  {
   "cell_type": "markdown",
   "metadata": {},
   "source": [
    "# q(Λ)\n",
    "$$\n",
    "\\begin{align}\n",
    "&\\ln q(\\boldsymbol{\\Lambda})=\\langle \\ln p(\\boldsymbol{Y}|\\boldsymbol{Z},\\boldsymbol{S},\\boldsymbol{\\Lambda},\\boldsymbol{R})\\rangle_{q(\\boldsymbol{Z},\\boldsymbol{S}),q(\\boldsymbol{R})}+\\ln p(\\boldsymbol{\\Lambda})+C\n",
    "\\\\\n",
    "&=\\sum_{t=1}^{T}\\sum_{k=1}^{K}\\sum_{d=1}^{D}−\\frac{1}{2}\\langle s_t^{k}\\{(y_{td} − \\boldsymbol{\\Lambda}_d^{(k)^T} \\boldsymbol{z}_t^{(k)})^2 R^{(k)}_d\\}\\rangle + (\\boldsymbol{\\Lambda}^{(k)}_d - \\boldsymbol{\\mu}_{\\Lambda_d}^{(k)})^T \\boldsymbol{\\Sigma}_{d}^{(k)^{-1}} (\\boldsymbol{\\Lambda}^{(k)}_d - \\boldsymbol{\\mu}_{\\Lambda_d}^{(k)})+C\n",
    "\\\\\n",
    "&= \\sum_{t=1}^{T}\\sum_{k=1}^{K}\\sum_{d=1}^{D}−\\frac{1}{2} \\{\\boldsymbol{\\Lambda}^{(k)^T}_d\\langle R_d^{(k)}\\rangle\\langle s_t^{(k)}\\boldsymbol{z}_d^{(k)}\\boldsymbol{z}_d^{(k)^T}\\rangle \\boldsymbol{\\Lambda}_d^{(k)}-2\\boldsymbol{\\Lambda}^{(k)^T}_d\\langle R_d^{(k)}\\rangle \\langle s_t^{(k)}\\boldsymbol{z}_d^{(k)^T}\\rangle + \\{\\boldsymbol{\\Lambda}^{(k)^T}_d \\boldsymbol{\\Sigma}_{\\Lambda_d}^{(k)^{-1}} \\boldsymbol{\\Lambda}_d^{(k)} -2\\boldsymbol{\\Lambda}_d^{(k)^{T}} \\boldsymbol{\\Sigma}_{\\Lambda_d}^{(k)^{-1}}\\boldsymbol{\\mu}_{\\Lambda_d}^{(k)}\\} + C\n",
    "\\\\\n",
    "&= \\sum_{t=1}^{T}\\sum_{k=1}^{K}\\sum_{d=1}^{D}−\\frac{1}{2} \\{\\boldsymbol{\\Lambda}^{(k)^T}_d (\\langle R_d^{(k)}\\rangle \\langle s_t^{(k)}\\boldsymbol{z}_d^{(k)}\\boldsymbol{z}_d^{(k)^T}\\rangle + \\boldsymbol{\\Sigma}_{\\Lambda_d}^{(k)^{-1}})\\boldsymbol{\\Lambda}_d^{(k)}-2\\boldsymbol{\\Lambda}^{(k)^T}_d (\\langle R_d^{(k)}\\rangle \\langle s_t^{(k)}\\boldsymbol{z}_d^{(k)}\\rangle\n",
    " + \\boldsymbol{\\Sigma}_{\\Lambda_d}^{(k)^{-1}}\\boldsymbol{\\mu}_{\\Lambda_d}^{(k)})\\} + C\n",
    " \\\\\n",
    " &=\\sum_{k=1}^{K}\\sum_{d=1}^{D} \\ln \\mathcal{N}(\\boldsymbol{\\Lambda}^{(k)^T}_d|\\hat{\\boldsymbol{\\mu}}_{\\Lambda_d}^{(k)},\\hat{\\boldsymbol{\\Sigma}}_{\\Lambda_d}^{(k)^{-1}})\n",
    "\\end{align}\n",
    "$$\n",
    "$$\n",
    "\\left\\{\\begin{align}\n",
    "\\hat{\\boldsymbol{\\Sigma}}_{\\Lambda_d}^{(k)^{-1}}&= \\langle R_d^{(k)}\\rangle \\sum_{t=1}^{T}\\langle s_t^{(k)}\\boldsymbol{z}_d^{(k)}\\boldsymbol{z}_d^{(k)^T}\\rangle + \\boldsymbol{\\Sigma}_{\\Lambda_d}^{(k)^{-1}}\n",
    "\\\\\n",
    "\\hat{\\boldsymbol{\\mu}}_{\\Lambda_d}^{(k)}&=\\hat{\\boldsymbol{\\Sigma}}_{\\Lambda_d}^{(k)}[\\langle R_d^{(k)}\\rangle \\sum_{t=1}^{T}\\langle s_t^{(k)}\\boldsymbol{z}_d^{(k)}\\rangle\n",
    " + \\boldsymbol{\\Sigma}_{\\Lambda_d}^{(k)^{-1}}\\boldsymbol{\\mu}_{\\Lambda_d}^{(k)}]\n",
    "\\end{align}\\right.\n",
    "$$"
   ]
  },
  {
   "cell_type": "markdown",
   "metadata": {},
   "source": [
    "# q(R)\n",
    "$$\n",
    "\\begin{align}\n",
    "&\\ln q(\\boldsymbol{R})=\\langle \\ln p(\\boldsymbol{Y}|\\boldsymbol{Z},\\boldsymbol{S},\\boldsymbol{\\Lambda},\\boldsymbol{R})\\rangle_{q(\\boldsymbol{Z},\\boldsymbol{S}),q(\\boldsymbol{\\Lambda})}+\\ln q(\\boldsymbol{R})+C\n",
    "\\\\\n",
    "&=\\sum_{t=1}^{T}\\sum_{k=1}^{K}\\sum_{d=1}^{D}−\\frac{1}{2}\\langle s_t^{(k)}\\{(y_{td} − \\boldsymbol{\\Lambda}_d^{(k)^T} \\boldsymbol{z}_t^{(k)})^2 R^{(k)}_d-\\ln R^{(k)}_d\\}\\rangle + \\sum_{k=1}^{K}\\sum_{d=1}^{D} (a_{R_d}^{(k)}-1)\\ln R_d^{(k)}-b_{R_d}^{(k)}R_d^{(k)}+C\n",
    "\\\\\n",
    "&=\\sum_{k=1}^{K}\\sum_{d=1}^{D} [(a_{R_d}^{(k)}+\\frac{1}{2}\\sum_{t=1}^{T}\\langle s_t^{(k)}\\rangle-1)\\ln R_d^{(k)}-\\{b_{R_d}^{(k)}+\\frac{1}{2}\\sum_{t=1}^{T}\\langle s_t^{(k)}(y_{td} − \\boldsymbol{\\Lambda}_d^{(k)^T} \\boldsymbol{z}_t^{(k)})^2 \\rangle\\}R_d^{(k)}]+C\n",
    "\\\\\n",
    "&=\\sum_{k=1}^{K}\\sum_{d=1}^{D} [(a_{R_d}^{(k)}+\\frac{1}{2}\\sum_{t=1}^{T}\\langle s_t^{(k)}\\rangle-1)\\ln R_d^{(k)}-\\{b_{R_d}^{(k)}+\\frac{1}{2}\\sum_{t=1}^{T}\\{\\langle s_t^{(k)}\\rangle y_{td}^2 - 2y_{td} \\langle \\boldsymbol{\\Lambda}_d^{(k)^T}\\rangle \\langle s_t^{(k)}\\boldsymbol{z}_t^{(k)}\\rangle +\\langle s_t^{(k)}(\\boldsymbol{\\Lambda}_d^{(k)^T} \\boldsymbol{z}_t^{(k)})^2 \\rangle\\}\\}R_d^{(k)}]+C\n",
    "\\\\\n",
    "&=\\sum_{k=1}^{K}\\sum_{d=1}^{D} (a_{R_d}^{(k)}+\\frac{1}{2}\\sum_{t=1}^{T}\\langle s_t^{(k)}\\rangle-1)\\ln R_d^{(k)}-[b_{R_d}^{(k)}+\\frac{1}{2}\\sum_{t=1}^{T}\\{\\langle s_t^{(k)}\\rangle y_{td}^2 - 2y_{td} \\langle \\boldsymbol{\\Lambda}_d^{(k)^T}\\rangle \\langle s_t^{(k)}\\boldsymbol{z}_t^{(k)}\\rangle +\\mathrm{Tr}(\\langle s_t^{(k)}\\boldsymbol{z}_t^{(k)}\\boldsymbol{z}_t^{(k)^T}\\rangle \\langle \\boldsymbol{\\Lambda}_d^{(k)}\\boldsymbol{\\Lambda}_d^{(k)^T} \\rangle\\} ] R_d^{(k)}+C\n",
    "\\\\\n",
    "&=\\sum_{k=1}^{K}\\sum_{d=1}^{D} \\mathrm{Gam}(R_d^{(k)}\\mid \\hat{a}_{R_d}^{(k)},\\hat{b}_{R_d}^{(k)})+C\n",
    "\\end{align}\n",
    "$$\n",
    "\n",
    "$$\n",
    "\\left\\{\\begin{align}\n",
    "\\hat{a}_{R_d}^{(k)} &= a_{R_d}^{(k)}+\\frac{1}{2}\\sum_{t=1}^{T}\\langle s_t^{(k)}\\rangle\n",
    "\\\\\n",
    "\\hat{b}_{R_d}^{(k)} &= b_{R_d}^{(k)}+\\frac{1}{2}\\sum_{t=1}^{T}\\{\\langle s_t^{(k)}\\rangle y_{d,t}^2 - 2y_{td} \\langle \\boldsymbol{\\Lambda}_d^{(k)^T}\\rangle \\langle s_t^{(k)}\\boldsymbol{z}_t^{(k)}\\rangle +\\mathrm{Tr}(\\langle s_t^{(k)}\\boldsymbol{z}_t^{(k)}\\boldsymbol{z}_t^{(k)^T}\\rangle \\langle \\boldsymbol{\\Lambda}_d^{(k)}\\boldsymbol{\\Lambda}_d^{(k)^T} \\rangle\\}\n",
    "\\end{align} \\right.\n",
    "$$"
   ]
  },
  {
   "cell_type": "markdown",
   "metadata": {},
   "source": [
    "$$\n",
    "\\begin{array}\n",
    "\\\\\n",
    "\\langle s_t^{(k)}(\\boldsymbol{\\Lambda}_d^{(k)^T} \\boldsymbol{z}_t^{(k)})^2 \\rangle\n",
    "& =\\langle s_t^{(k)}(\\boldsymbol{\\Lambda}_d^{(k)^T} \\boldsymbol{z}_t^{(k)})(\\boldsymbol{\\Lambda}_d^{(k)^T} \\boldsymbol{z}_t^{(k)}) \\rangle\n",
    "\\\\\n",
    "&=\\langle s_t^{(k)}(\\boldsymbol{\\Lambda}_d^{(k)^T} \\boldsymbol{z}_t^{(k)})(\\boldsymbol{z}_t^{(k)^T}\\boldsymbol{\\Lambda}_d^{(k)}) \\rangle\n",
    "\\\\\n",
    "&=\\langle \\boldsymbol{\\Lambda}_d^{(k)^T} (s_t^{(k)}\\boldsymbol{z}_t^{(k)}\\boldsymbol{z}_t^{(k)^T}) \\boldsymbol{\\Lambda}_d^{(k)} \\rangle \n",
    "\\\\\n",
    "&= \\mathrm{Tr}[\\langle s_t^{(k)}\\boldsymbol{z}_t^{(k)}\\boldsymbol{z}_t^{(k)^T}\\rangle \\langle \\boldsymbol{\\Lambda}_d^{(k)}\\boldsymbol{\\Lambda}_d^{(k)^T} \\rangle ]\n",
    "\\\\\n",
    "\\\\\n",
    "A^TBC=\\mathrm{Tr}(BAC^T)\n",
    "\\end{array}\n",
    "$$"
   ]
  },
  {
   "cell_type": "markdown",
   "metadata": {},
   "source": [
    "# q(π)\n",
    "$$\n",
    "\\begin{align}\n",
    "\\ln q(\\boldsymbol{\\pi})&=\\langle\\ln p(\\boldsymbol{S}|\\boldsymbol{\\pi})\\rangle_{q(\\boldsymbol{S})}+\\ln p(\\boldsymbol{\\pi}) +C\n",
    "\\\\\n",
    "&=\\sum_{t=1}^{T} \\sum_{k=1}^{K} \\langle s_t^{(k)}\\rangle \\ln\\pi^{(k)} + \\sum_{k=1}^{K}(\\alpha_{\\pi}^{(k)} − 1)\\ln\\pi^{(k)} + C\n",
    "\\\\\n",
    "&=\\sum_k^K(\\sum_t^T\\langle s_t^{(k)}\\rangle +\\alpha_{\\pi}^{(k)}−1)\\ln\\pi^{(k)}+C\n",
    "\\\\\n",
    "&=\\ln\\mathrm{Dir}(\\pi|\\hat{\\alpha}_{\\pi})\n",
    "\\end{align}\n",
    "$$\n"
   ]
  }
 ],
 "metadata": {
  "kernelspec": {
   "display_name": "Python 3",
   "language": "python",
   "name": "python3"
  },
  "language_info": {
   "codemirror_mode": {
    "name": "ipython",
    "version": 3
   },
   "file_extension": ".py",
   "mimetype": "text/x-python",
   "name": "python",
   "nbconvert_exporter": "python",
   "pygments_lexer": "ipython3",
   "version": "3.6.9"
  }
 },
 "nbformat": 4,
 "nbformat_minor": 2
}
